classes_parte2/ArvoreBinariaBusca.dfy
@@ -1,0 +1,105 @@
+datatype Option<T> = None | Some(T)
+
+ghost predicate Menor(a:set<int>, b:set<int>) {
+  forall x, y :: x in a && y in b ==> x < y
+}
+
+ghost function Uniao<Data>(m:map<int, Data>, n:Nodo?<Data>): map<int, Data>
+  reads n
+{
+  if n == null
+  then m
+  else m + n.Mapa
+}
+
+class Nodo<T>
+{
+  //Abstração
+  ghost var Mapa:map<int,T>
+  ghost var Repr:set<object>
+  //Implementação
+  var chave:int
+  var valor:T
+  var esq:Nodo?<T>
+  var dir:Nodo?<T>
+
+  ghost predicate Valid()
+    reads this, Repr
+    ensures Valid() ==> this in Repr
+  {
+    && this in Repr
+    && (esq != null ==>
+      && esq in Repr
+      && esq.Repr <= Repr
+      && this !in esq.Repr
+      && esq.Valid()
+      && Menor(esq.Mapa.Keys, {chave})
+    )
+    && (dir != null ==>
+      && dir in Repr
+      && dir.Repr <= Repr
+      && this !in dir.Repr
+      && dir.Valid()
+      && Menor({chave}, dir.Mapa.Keys)
+    )
+    && (esq != null && dir != null ==> esq.Repr !! dir.Repr)
+    && Mapa == Uniao(Uniao(map[chave := valor], esq), dir)
+  }
+
+  constructor (chave:int, valor:T)
+    ensures Valid() && fresh(Repr)
+    ensures Mapa == map[chave := valor]
+
+  function Buscar(chave:int):Option<T>
+    requires Valid()
+    reads Repr
+    ensures chave in Mapa.Keys ==> Buscar(chave) == Some(Mapa[chave])
+    ensures chave !in Mapa.Keys ==> Buscar(chave) == None
+
+  method Adicionar(chave:int, valor:T)
+    requires Valid()
+    modifies Repr
+    ensures Valid() && fresh(Repr - old(Repr))
+    ensures Mapa == old(Mapa)[chave := valor]
+
+}
+
+class ArvoreBinariaBusca<T>
+{
+  //Abstração
+  ghost var Mapa:map<int,T>
+  ghost var Repr:set<object>
+  //Implementação
+  var raiz:Nodo?<T>
+
+  ghost predicate Valid()
+    reads this, Repr
+    ensures Valid() ==> this in Repr
+  {
+    && this in Repr
+    && (|Mapa.Keys| == 0 ==> raiz == null)
+    && (|Mapa.Keys| != 0 ==>
+      && raiz in Repr
+      && raiz.Repr <= Repr
+      && this !in raiz.Repr
+      && raiz.Valid()
+      && raiz.Mapa == Mapa
+    )
+  }
+    
+  constructor ()
+    ensures Valid() && fresh(Repr)
+    ensures Mapa == map[]
+    
+  function Buscar(chave:int):Option<T>
+    requires Valid()
+    reads Repr
+    ensures chave in Mapa.Keys ==> Buscar(chave) == Some(Mapa[chave])
+    ensures chave !in Mapa.Keys ==> Buscar(chave) == None
+    
+  method Adicionar(chave:int, valor:T)
+    requires Valid()
+    modifies Repr
+    ensures Valid() && fresh(Repr - old(Repr))
+    ensures Mapa == old(Mapa)[chave := valor]
+}
