classes_parte2/ListaIndutiva.dfy
@@ -1,0 +1,33 @@
+datatype list<T> =
+  | Nil
+  | Cons(hd: T, tl: list)
+
+function tamanho<T>(l: list): nat
+{
+  match l
+  {
+    case Nil => 0
+    case Cons(h,t) => 1 + tamanho(t)
+  }
+}
+
+function concatenar<T>(l1: list, l2: list): list
+{
+  match l1 {
+    case Nil => l2
+    case Cons(h,t) => Cons(h,concatenar(t,l2))
+  }
+}
+
+function inverter<T>(l:list):list
+{
+    inverterAux(l,Nil)
+}
+
+function inverterAux<T>(l: list, acc: list): list
+{
+  match l {
+    case Nil => acc
+    case Cons(h,t) => inverterAux(t,Cons(h,acc))
+  }
+}
